more

Ordered_Resolution_Prover/Executable_Subsumption.thy
@@ -12,144 +12,92 @@ theory Executable_Subsumption
     "$ISAFOR/Rewriting/Matching"
 begin
 
-definition "ext_gsubst x = Fun (Inr x) []"
-definition "ext_emb = map_term Inl id"
-
-fun undo_ext where
-  "undo_ext (Var x) = Var x"
-| "undo_ext (Fun (Inr x) ts) = Var x"
-| "undo_ext (Fun (Inl x) ts) = Fun x (map undo_ext ts)"
-
-lemma undo_ext_gsubst_inverse[simp]:
-  "undo_ext (ext_gsubst x) = Var x"
-  "undo_ext (ext_emb t \<cdot> \<sigma>) = t \<cdot> (undo_ext o \<sigma>)"
-  "undo_ext (ext_emb t) = t"
-  by (induct t) (auto simp: ext_gsubst_def ext_emb_def cong: map_cong)
-
-lemma subst_ext_gsubst: "t \<cdot> ext_gsubst \<cdot> \<sigma> = t \<cdot> ext_gsubst"
-  by (induct t) (auto simp: ext_gsubst_def)
-
-lemma is_ground_subst_ext_gsubst: "is_ground_subst ext_gsubst"
-  unfolding is_ground_subst_def ext_gsubst_def is_ground_atm_def subst_ext_gsubst by blast
-
-lemma ext_emb_subst[simp]: "ext_emb (t \<cdot> \<sigma>) = ext_emb t \<cdot> (ext_emb o \<sigma>)"
-  by (induct t) (auto simp: ext_emb_def)
-
-lemma subsumes_ground:
-  "subsumes (map_clause ext_emb C) (map_clause ext_emb D \<cdot>cls ext_gsubst) \<longleftrightarrow> subsumes C D"
-  (is "?L \<longleftrightarrow> ?R")
-proof
-  assume ?R
-  then obtain \<sigma> where "subst_cls C \<sigma> \<subseteq># D"
-    unfolding subsumes_def by auto
-  from image_mset_subseteq_mono[of _ _ "map_literal ((\<lambda>t. t \<cdot> ext_gsubst) o ext_emb)", OF this]
-  show ?L
-    by (auto simp: subsumes_def multiset.map_comp literal.map_comp
-     subst_cls_def subst_apply_clause_def subst_lit_def o_def subst_subst subst_compose_def)
-qed (auto simp: subsumes_def multiset.map_comp literal.map_ident literal.map_comp
-     subst_cls_def subst_apply_clause_def subst_lit_def o_def
-     dest!: image_mset_subseteq_mono[of _ _ "map_literal undo_ext"])
-
 context notes length_remove1[termination_simp] find_Some_iff[termination_simp] begin
 fun subsumes_list where
-  "subsumes_list [] Ks = Some Var"
-| "subsumes_list (L # Ls) Ks =
-     (case List.find (\<lambda>K. is_pos K = is_pos L \<and> match (atm_of K) (atm_of L) \<noteq> None) Ks of
-       None \<Rightarrow> None
+  "subsumes_list [] Ks \<sigma> = True"
+| "subsumes_list (L # Ls) Ks \<sigma> =
+     (case List.find (\<lambda>K. is_pos K = is_pos L \<and> match_term_list [(atm_of L, atm_of K)] \<sigma> \<noteq> None) Ks of
+       None \<Rightarrow> False
      | Some K \<Rightarrow>
-         (let \<rho> = the (match (atm_of K) (atm_of L)); Ks' = remove1 K Ks in
-         case subsumes_list (map (\<lambda>L. L \<cdot>lit \<rho>) Ls) Ks' of
-           None \<Rightarrow> subsumes_list (L # Ls) Ks'
-         | Some \<sigma> \<Rightarrow> Some (\<rho> \<circ>\<^sub>s \<sigma>)))"
+         (let \<rho> = the (match_term_list [(atm_of L, atm_of L)] \<sigma>); Ks' = remove1 K Ks in
+         subsumes_list Ls Ks' \<rho> \<or> subsumes_list (L # Ls) Ks' \<rho>))"
 end
 
 declare subsumes_list.simps(2)[simp del]
 
 lemma atm_of_map_literal[simp]: "atm_of (map_literal f l) = f (atm_of l)"
+  by (cases l; simp)
 
-abbreviation subsumes_list_subst  (infixl "\<triangleleft>" 60) where
-  "subsumes_list_subst Ls Ks \<equiv> subsumes (mset Ls) (mset Ks)"
-term match_term_list
-lemma "\<forall>K \<in> set Ks. is_ground_lit K \<Longrightarrow>
-  L # Ls \<triangleleft> Ks \<longleftrightarrow> (\<exists>K \<in> set Ks. \<exists>\<rho>. L \<cdot>lit \<rho> = K \<and> map (\<lambda>L. L \<cdot>lit \<rho>) Ls \<triangleleft> remove1 K Ks)"
-  unfolding subsumes_def
+definition "extends_subst \<sigma> \<tau> = (\<forall>x \<in> dom \<sigma>. \<sigma> x = \<tau> x)"
+
+lemma extends_subst_refl: "extends_subst \<sigma> \<sigma>"
+  unfolding extends_subst_def by auto
+
+lemma extends_subst_trans: "extends_subst \<sigma> \<tau> \<Longrightarrow> extends_subst \<tau> \<rho> \<Longrightarrow> extends_subst \<sigma> \<rho>"
+  unfolding extends_subst_def dom_def by (metis mem_Collect_eq)
+
+lemma extends_subst_dom: "extends_subst \<sigma> \<tau> \<Longrightarrow> dom \<sigma> \<subseteq> dom \<tau>"
+  unfolding extends_subst_def dom_def by auto
+
+lemma extends_subst_empty: "extends_subst Map.empty \<tau>"
+  unfolding extends_subst_def by auto
+
+lemma extends_subst_cong_term:
+  "extends_subst \<sigma> \<tau> \<Longrightarrow> vars_term t \<subseteq> dom \<sigma> \<Longrightarrow> t \<cdot> subst_of_map Var \<sigma> = t \<cdot> subst_of_map Var \<tau>"
+  by (force simp: extends_subst_def subst_of_map_def split: option.splits intro!: term_subst_eq)
+
+lemma extends_subst_cong_lit:
+  "extends_subst \<sigma> \<tau> \<Longrightarrow> vars_lit L \<subseteq> dom \<sigma> \<Longrightarrow> L \<cdot>lit subst_of_map Var \<sigma> = L \<cdot>lit subst_of_map Var \<tau>"
+  by (cases L) (auto simp: extends_subst_cong_term)
+
+definition "subsumes_modulo C D \<sigma> =
+   (\<exists>\<tau>. vars_clause C \<subseteq> dom \<tau> \<and> extends_subst \<sigma> \<tau> \<and> subst_cls C (subst_of_map Var \<tau>) \<subseteq># D)"
+
+abbreviation subsumes_list_modulo where
+  "subsumes_list_modulo Ls Ks \<sigma> \<equiv> subsumes_modulo (mset Ls) (mset Ks) \<sigma>"
+
+lemma vars_clause_add_mset[simp]: "vars_clause (add_mset L C) = vars_lit L \<union> vars_clause C"
+  unfolding vars_clause_def by auto
+
+lemma subsumes_list_modulo_Cons: "subsumes_list_modulo (L # Ls) Ks \<sigma> \<longleftrightarrow>
+  (\<exists>K \<in> set Ks. \<exists>\<tau>. extends_subst \<sigma> \<tau> \<and> vars_lit L \<subseteq> dom \<tau> \<and> L \<cdot>lit (subst_of_map Var \<tau>) = K
+     \<and> subsumes_list_modulo Ls (remove1 K Ks) \<tau>)"
+  unfolding subsumes_modulo_def
   apply safe
-  apply (auto simp: insert_subset_eq_iff subst_lit_def subst_cls_def literal.map_ident) []
-   apply (erule bexI[rotated])
-   apply (rule exI conjI)+
-    apply (rule refl)
-   apply (rule exI[of _ Var])
-   apply (auto simp: subst_cls_def subst_lit_def literal.map_ident) []
-  apply (rule_tac x = "\<rho> \<circ>\<^sub>s \<sigma>" in exI)
-  apply (auto simp: insert_subset_eq_iff subst_lit_def subst_cls_def
-    cong: literal.map_cong split: if_splits)
-  
-  find_theorems "add_mset _ _ \<subseteq># _"
-  sorry
+   apply (auto simp: insert_subset_eq_iff subst_lit_def subst_cls_def literal.map_ident
+     intro: extends_subst_refl extends_subst_trans)
+  apply (intro exI conjI)
+      prefer 3
+      apply (rule extends_subst_trans; assumption)
+     apply (erule (1) order_trans[OF _ extends_subst_dom])
+    apply assumption
+  apply (auto simp: extends_subst_cong_lit)
+  done
 
-lemma subsumes_list_complete:
-  "subsumes_list Ls Ks = None \<Longrightarrow> \<not> Ls \<triangleleft> Ks"
-  sorry
-proof (induction Ls Ks rule: subsumes_list.induct[case_names Nil_Nil Cons_Nil Cons])
-  case (Cons L Ls Ks)
-  show ?case sorry(*
-  proof
-    fix \<rho>
-    from Cons.prems show "\<not> mset (map (\<lambda>a. a \<cdot>lit \<rho>) (L # Ls)) \<subseteq># mset Ks"
-    proof (cases "find (\<lambda>K. is_pos K = is_pos L \<and> match (atm_of K) (atm_of L) \<noteq> None) Ks")
-      case None
-      then show ?thesis
-        by (auto simp: find_None_iff dest!: spec[of _ "L \<cdot>lit \<rho>"] match_complete)
-    next
-      case (Some K)
-      let ?\<rho>KL = "the (match (atm_of K) (atm_of L))"
-      let ?Ks = "remove1 K Ks"
-      from Cons.prems Some show ?thesis
-      proof (cases "subsumes_list (map (\<lambda>L. L \<cdot>lit ?\<rho>KL) Ls) ?Ks")
-        case None
-        with Cons.prems Some have "subsumes_list (L # Ls) ?Ks = None"
-          by (subst (asm) subsumes_list.simps(2)) (auto simp: Let_def)
-        note IH =
-          Cons.IH(1)[OF Some refl refl None, THEN spec, of \<rho>]
-          Cons.IH(2)[OF Some refl refl None this, THEN spec, of \<rho>]
-        with Some None show ?thesis
-          apply (auto simp: literal.map_comp o_def insert_subset_eq_iff is_pos_def
-            find_Some_iff subst_subst simp del: subst_subst_compose dest!: match_sound spec[of _ "\<rho>"])
-          sledgehammer
-          subgoal for i \<sigma> t
-           apply (drule spec[of _ "\<rho>"])
-            apply (erule notE)
-            apply auto
-          find_theorems "add_mset _ _ \<subseteq># _"
-          sorry
-        sorry
-      qed (subst (asm) subsumes_list.simps(2), auto)
-    qed
-  qed*)
-qed simp
-
-lemma subsumes_list_sound:
-  "subsumes_list Ls Ks = Some \<rho> \<Longrightarrow> mset (map (\<lambda>L. L \<cdot>lit \<rho>) Ls) \<subseteq># mset Ks"
-  sorry
-(*
-proof (induct Ls Ks arbitrary: \<rho> rule: subsumes_list.induct[case_names Nil Cons])
-  case (Cons L Ls Ks)
-  then show ?case sorry
-qed simp
-*)
+lemma subsumes_list_alt:
+  "subsumes_list Ls Ks \<sigma> \<longleftrightarrow> subsumes_list_modulo Ls Ks \<sigma>"
+proof (induction Ls Ks \<sigma> rule: subsumes_list.induct[case_names Nil Cons])
+  case (Cons L Ls Ks \<sigma>)
+  then show ?case
+    apply (auto simp: subsumes_list_modulo_Cons subsumes_list.simps(2)[of L Ls Ks]
+      find_None_iff Let_def
+      split: option.splits) sorry
+qed (auto simp: subsumes_modulo_def subst_cls_def vars_clause_def intro: extends_subst_refl) 
 
 lemma subsumes_subsumes_list[code_unfold]:
-  "subsumes (mset Ls) (mset Ks) = (subsumes_list Ls Ks \<noteq> None)"
-  using subsumes_list_sound[of Ls Ks] subsumes_list_complete[of Ls Ks]
-  by (auto simp: subst_cls_def subst_lit_def subsumes_def)
-
-lemma subsumes_list_subsumes:
-  "(\<exists>\<sigma>. subsumes_list Ls Ks = Some \<sigma>) = subsumes (mset Ls) (mset Ks)"
-  "(subsumes_list Ls Ks = None) = (\<not> subsumes (mset Ls) (mset Ks))"
-  by (simp_all add: subsumes_subsumes_list)
+  "subsumes (mset Ls) (mset Ks) = subsumes_list Ls Ks Map.empty"
+unfolding subsumes_list_alt[of Ls Ks Map.empty]
+proof
+  assume "subsumes (mset Ls) (mset Ks)"
+  then obtain \<sigma> where "subst_cls (mset Ls) \<sigma> \<subseteq># mset Ks" unfolding subsumes_def by blast
+  moreover define \<tau> where "\<tau> = Some o \<sigma>"
+  ultimately show "subsumes_list_modulo Ls Ks Map.empty"
+    unfolding subsumes_modulo_def
+    by (auto intro!: exI[of _ \<tau>] simp: extends_subst_empty subst_of_map_def[abs_def])
+qed (auto simp: subsumes_modulo_def extends_subst_empty subst_lit_def subsumes_def)
 
 lemma strictly_subsumes_subsumes_list[code_unfold]:
-  "strictly_subsumes (mset Ls) (mset Ks) = (subsumes_list Ls Ks \<noteq> None \<and> subsumes_list Ks Ls = None)"
+  "strictly_subsumes (mset Ls) (mset Ks) = (subsumes_list Ls Ks Map.empty \<and> \<not> subsumes_list Ks Ls Map.empty)"
   unfolding strictly_subsumes_def subsumes_subsumes_list by simp
 
 end
